\documentclass[xcolor=x11names,compress]{beamer}
\usepackage[english]{babel}

%% General document %%%%%%%%%%%%%%%%%%%%%%%%%%%%%%%%%%
\usepackage{graphicx}
\usepackage{tikz}
\usepackage{wrapfig}
\usepackage{hyperref}

\usetikzlibrary{decorations.fractals}
%%%%%%%%%%%%%%%%%%%%%%%%%%%%%%%%%%%%%%%%%%%%%%%%%%%%%%


%% Beamer Layout %%%%%%%%%%%%%%%%%%%%%%%%%%%%%%%%%%
\useoutertheme[subsection=false,shadow]{miniframes}
\useinnertheme{default}
\usefonttheme{serif}
\usepackage{palatino}

\setbeamerfont{title like}{shape=\scshape}
\setbeamerfont{frametitle}{shape=\scshape}

\setbeamercolor*{lower separation line head}{bg=DeepSkyBlue4} 
\setbeamercolor*{normal text}{fg=black,bg=white} 
\setbeamercolor*{alerted text}{fg=red} 
\setbeamercolor*{example text}{fg=black} 
\setbeamercolor*{structure}{fg=black} 
 
\setbeamercolor*{palette tertiary}{fg=black,bg=black!10} 
\setbeamercolor*{palette quaternary}{fg=black,bg=black!10} 

\renewcommand{\(}{\begin{columns}}
\renewcommand{\)}{\end{columns}}
\newcommand{\<}[1]{\begin{column}{#1}}
\renewcommand{\>}{\end{column}}
%%%%%%%%%%%%%%%%%%%%%%%%%%%%%%%%%%%%%%%%%%%%%%%%%%
\newcommand{\hlb}[1]{\textbf{\textcolor{blue}{#1}}}
\newcommand{\hl}[1]{\textcolor{blue}{#1}}
\newcommand{\lien}[2]{\mathcal{L}_{#1}^{#2}}
\newcommand{\lie}[1]{\mathcal{L}_{#1}}

\newcommand{\colv}[2]{\begin{pmatrix}#1\\#2\end{pmatrix}}

%\usepackage[english]{babel}
\usepackage[utf8]{inputenc}
%\usetheme{Goettingen}

\begin{document}
\title{Bifurcations in continuous time dynamical systems}
\author{Debsankha Manik}

\begin{frame}

%opening

\titlepage

\end{frame}


\section{Vanishing chaos}
\begin{frame}{Vanishing chaos}
When $\frac{2\omega_g}{\omega}$ is an integer, no chaos is observed at grazing:
\begin{figure}
\begin{center}
\includegraphics[width=0.9\columnwidth]{chaos-vanish-m-2}
\end{center}
\end{figure}
\end{frame}

\begin{frame}
\section{Alternate approach to ZDM}
Suppose the parameters of the system are set such that 
$\frac{F}{\sqrt{(\omega_0^2-\omega^2)^2+\omega^2\gamma^2}}=F_g(\omega_0,\omega,\gamma,F)=\sigma$
. This constitutes a steady state grazing orbit.  \\
 \vspace{1em}

Suppose we look at stroboscopic time slices such that the grazing orbit grazes 
the boundary at $t=\tau$.  \\
\vspace{1em}

Now we perturb the system slightly so that the system hits the boundary with 
some non zero velocity at $t=\tau+\delta t$\\

\begin{eqnarray*}
\colv{x(0)}{v(0)}&=&\colv{x_p(0)}{v_p(0)}+\colv{x_h(0)}{v_h(0)}\\
\colv{x(\tau+\delta t)}{v(\tau+\delta t)}&=&\colv{x_p(\tau+\delta t)}{v_p(\tau+\delta t)}+\colv{x_h(\tau+\delta t)}{v_h(\tau+\delta t)}
\end{eqnarray*}
\end{frame}

\begin{frame}[label=BackFromM]
After collision:\\
\begin{eqnarray*}
\colv{x}{v}&=&\colv{x_p(\tau+\delta t)}{-v_p(\tau+\delta t)}+\colv{x_h(\tau+\delta t)}{-v_h(\tau+\delta t)}\\
&=&\colv{x_p(\tau+\delta t)}{v_p(\tau+\delta t)}+\colv{x_h(\tau+\delta t)}{v_h(\tau+\delta t)}\\
&&+\colv{0}{-2v_h(\tau+\delta t)-2v_p(\tau+\delta t)}
\end{eqnarray*}

\begin{eqnarray*}
\colv{x(T)}{v(T)}&=&\vec{x_p}(T)+M(T-\tau-\delta 
t)\left\{\colv{x_h(\tau+\delta t)}{v_h(\tau+\delta t)}\right.\\
&&\left.+\colv{0}{-2v_h(\tau+\delta t)-2v_p(\tau+\delta t)}\right\}\\
&=&\vec{x_p}(T)+M(T)\vec{x_h}(0)\\&&+M(T-\tau-\delta t)\colv{0}{-2v_p(\tau+\delta t)-2v_h(\tau+\delta t)}
\end{eqnarray*}
\hyperlink{homogen-evol}{\beamergotobutton{Expand M}}

\end{frame}

\begin{frame}[label=poincare_slide]
Therefore we have our Poincare map:
\begin{equation}
\label{poincare-hardcol}
\vec{x'}(T)=M(T)\vec{x'}(0)+M(T-\tau-\delta t)\colv{0}{-2v_p(\tau+\delta t)-2v_h(\tau+\delta t)}
\end{equation}

\hyperlink{new_poincare_slide}{\beamergotobutton{back}}
$\left\{\vec{x'}(t)=\vec{x}(t)-\vec{x_p}(t)\right\}$

If we can find expressions for $\delta t, v_p, v_h$ in terms of $x(0),v(0)$, 
the job will be done.  
\end{frame}

\begin{frame}
Recall:
\[
x_p(\tau)=\frac{F}{\sqrt{(\omega_0^2-\omega^2)^2+\omega^2\gamma^2}}:=x_m
\]
\[
v_p(\tau)=0
\]

We have:
\begin{eqnarray*}
x_h(\tau+\delta t)+x_p(\tau+\delta t)&=&\sigma\\
x_h(\tau)+\dot{x}(\tau)\delta t+x_m\cos{\omega \delta t}&=&\sigma\\
x_h(\tau)+\dot{x}(\tau)\delta t+x_m\left(1-\frac{(\omega \delta t)^2}{2}\right)&=&\sigma
\end{eqnarray*}

The root of this equation gives the value of $\delta t$
(If the roots happen to be complex, it means no collision will take place)
\end{frame}

\begin{frame}
$v_h$ and $v_p$ are calculated in a similar fashion:
\[
v_p(\tau+\delta t)=-x_m\omega\sin{\omega\delta t}
\]

\begin{eqnarray*}
v_h(\tau+\delta t)&=&v_h(\tau)+\dot{v_h}(\tau)\delta t\\
&=&v_h(\tau)+\delta t(-\gamma v_h(\tau)-w_0^2x_h(\tau))
\end{eqnarray*}

This map should show all the bifurcations shown by the continuous time system.  
\end{frame}


\begin{frame}
\begin{figure}
\caption{}
\begin{center}
\includegraphics[width=0.9\columnwidth]{poinc-bf-f}
\end{center}
\end{figure}
\end{frame}

\begin{frame}[label=homogen-evol]
\begin{eqnarray}
M(t)=\frac{e^{-\gamma t/2}}{\omega_g}
\begin{pmatrix}
\omega_g\cos{\omega_g t}+\frac{\gamma}{2}\sin{\omega_g t} & \sin{\omega_g t}\\
-k\sin{\omega_g t} & \omega_g\cos{\omega_g t}-\frac{\gamma}{2}\sin{\omega_g t}
\end{pmatrix}
\end{eqnarray}

$(\omega_g=\frac{\sqrt{4k-\gamma^2}}{2})$
\hyperlink{BackFromM}{\beamergotobutton{Back}}
\end{frame}

\begin{frame}[label=new_poincare_slide]
We derived an exact expression for the poincare map sometime ago.  
\hyperlink{poincare_slide}{\beamergotobutton{Exact formula}}
Let the parameters be such that the stable orbit grazes slightly:
$x_m(\left\{parameters\right\})=\sigma+\varepsilon$.  \\

Now start from an initial condition such that $\left|x'(0)\right|=0$.  
(Exactly on the stable orbit).\\

Then we have:
\begin{align*}
x_mcos\left(\omega \tau+tan^{-1}\frac{\omega \gamma}{\omega^2-\omega_0^2}\right)&=\sigma\\
\omega \tau+tan^{-1}\frac{\omega \gamma}{\omega^2-\omega_0^2}&=cos^{-1}\left(1+\frac{\varepsilon}{\sigma}\right)^{-1}\\
&\approx2n\pi+\sqrt{\frac{2\varepsilon}{\sigma}}\\
\tau&\approx \frac{1}{\omega}\left(2\pi+\sqrt{\frac{2\varepsilon}{\sigma}}-tan^{-1}\frac{\omega \gamma}{\omega^2-\omega_0^2}\right)
\end{align*}
\end{frame}

\begin{frame}
Now suppose $0<|x'(0)|<<1$.   
Let the time of collision $t_c=\tau+\delta t$
\begin{align*}
x_mcos\left(\omega (\tau+\delta t)+tan^{-1}\frac{\omega 
\gamma}{\omega^2-\omega_0^2}\right)+x_h(\tau+\delta t)&=\sigma\\
x_mcos\left(\left(\omega \tau+tan^{-1}\frac{\omega 
\gamma}{\omega^2-\omega_0^2}\right)+\omega \delta t\right)+x_h(\tau+\delta t)&=\sigma\\
\sigma-\omega x_m\delta t sin\left(\omega \tau+tan^{-1}\frac{\omega 
\gamma}{\omega^2-\omega_0^2}\right)+x_h(\tau+\delta t)&=\sigma\\
-\omega \delta tx_m\sqrt{1-(\sigma/x_m)^2}+x_h(\tau+\delta t)&=0\\
\frac{x_h(\tau)}{\omega\sqrt{x_m^2-\sigma^2}-v_h(\tau)}&=\delta t
\end{align*}
\end{frame}

\begin{frame}
\begin{align*}
v_p(\tau+\delta t)&=-\omega x_m sin\left( \omega (\tau+\delta t)+tan^{-1}\frac{\omega 
\gamma}{\omega^2-\omega_0^2}\right)\\
&=-\omega x_m sin\left( 
2\pi+\sqrt{\frac{2\varepsilon}{\sigma}}-tan^{-1}\frac{\omega 
\gamma}{\omega^2-\omega_0^2}+\omega \delta t + tan^{-1}\frac{\omega 
\gamma}{\omega^2-\omega_0^2} \right)\\
&=-\omega x_m sin\left(\omega\delta t+\sqrt{\frac{2\varepsilon}{\sigma}}\right) 
\end{align*}
\end{frame}
\end{document}
